2016/Lambda_calculus.thy
@@ -1,7 +1,8 @@
 theory Lambda_calculus
-  imports Main
-          List_extra
-          "$AFP/List-Index/List_Index"
+imports
+  Main
+  List_extra
+  "List-Index.List_Index"
 begin
 
 datatype ltype =
